System transition: IC Management Canister: Code upgrade [DONE]

theories/IC.thy
@@ -158,6 +158,8 @@ typedef ('p, 'canid, 'b, 'w, 'sm, 'c, 's) canister_module =
 setup_lifting type_definition_canister_module
 
 lift_definition canister_module_init :: "('p, 'canid, 'b, 'w, 'sm, 'c, 's) canister_module \<Rightarrow> 'canid \<times> 'b arg \<times> 'p \<times> 'b env \<Rightarrow> trap_return + 'w cycles_return" is "init" .
+lift_definition canister_module_pre_upgrade :: "('p, 'canid, 'b, 'w, 'sm, 'c, 's) canister_module \<Rightarrow> 'w \<times> 'p \<times> 'b env \<Rightarrow> trap_return + 'sm cycles_return" is pre_upgrade .
+lift_definition canister_module_post_upgrade :: "('p, 'canid, 'b, 'w, 'sm, 'c, 's) canister_module \<Rightarrow> 'canid \<times> 'sm \<times> 'b arg \<times> 'p \<times> 'b env \<Rightarrow> trap_return + 'w cycles_return" is post_upgrade .
 
 lift_definition dispatch_method :: "'s \<Rightarrow> ('p, 'canid, 'b, 'w, 'sm, 'c, 's) canister_module \<Rightarrow>
   ((('b arg \<times> 'p \<times> 'b env \<times> available_cycles) \<Rightarrow> ('w, 'p, 'canid, 's, 'b, 'c) update_func) +
@@ -1013,9 +1015,8 @@ definition ic_code_installation_pre :: "nat \<Rightarrow> ('p, 'uid, 'canid, 'b,
     (case (candid_parse_text d [encode_string ''mode''], candid_parse_blob d [encode_string ''wasm_module''], candid_parse_blob d [encode_string ''arg'']) of
       (Some mode, Some w, Some a) \<Rightarrow>
     (case parse_wasm_mod w of Some m \<Rightarrow>
-    (case list_map_get (controllers S) cid of Some ctrls \<Rightarrow>
-    (case (list_map_get (time S) cid, list_map_get (balances S) cid, list_map_get (canister_status S) cid) of
-      (Some t, Some bal, Some can_status) \<Rightarrow>
+    (case (list_map_get (controllers S) cid, list_map_get (time S) cid, list_map_get (balances S) cid, list_map_get (canister_status S) cid) of
+      (Some ctrls, Some t, Some bal, Some can_status) \<Rightarrow>
       let env = \<lparr>env_time = t, balance = bal, freezing_limit = ic_freezing_limit S cid, certificate = None, status = simple_status can_status\<rparr> in
       ((mode = encode_string ''install'' \<and> (case list_map_get (canisters S) cid of Some None \<Rightarrow> True | _ \<Rightarrow> False)) \<or> mode = encode_string ''reinstall'') \<and>
       cer \<in> ctrls \<and>
@@ -1023,7 +1024,7 @@ definition ic_code_installation_pre :: "nat \<Rightarrow> ('p, 'uid, 'canid, 'b,
       | Inr ret \<Rightarrow> cycles_return.cycles_used ret \<le> bal) \<and>
       parse_public_custom_sections w \<noteq> None \<and>
       parse_private_custom_sections w \<noteq> None
-    | _ \<Rightarrow> False) | _ \<Rightarrow> False) | _ \<Rightarrow> False) | _ \<Rightarrow> False) | _ \<Rightarrow> False)
+    | _ \<Rightarrow> False) | _ \<Rightarrow> False) | _ \<Rightarrow> False) | _ \<Rightarrow> False)
   | _ \<Rightarrow> False))"
 
 definition ic_code_installation_post :: "nat \<Rightarrow> nat \<Rightarrow> ('p, 'uid, 'canid, 'b, 'w, 'sm, 'c, 's, 'cid, 'pk) ic \<Rightarrow> ('p, 'uid, 'canid, 'b, 'w, 'sm, 'c, 's, 'cid, 'pk) ic" where
@@ -1073,6 +1074,81 @@ proof -
     by (auto simp: ic_code_installation_pre_def ic_code_installation_post_def ic_code_installation_burned_cycles_def total_cycles_def Let_def msgs list_map_sum_in[where ?f="balances S"] split: message.splits option.splits sum.splits prod.splits)
 qed
 
+
+
+(* System transition: IC Management Canister: Code upgrade [DONE] *)
+
+definition ic_code_upgrade_pre :: "nat \<Rightarrow> ('p, 'uid, 'canid, 'b, 'w, 'sm, 'c, 's, 'cid, 'pk) ic \<Rightarrow> bool" where
+  "ic_code_upgrade_pre n S = (n < length (messages S) \<and> (case messages S ! n of Call_message orig cer cee mn d trans_cycles q \<Rightarrow>
+    (q = Unordered \<or> (\<forall>j < n. message_queue (messages S ! j) \<noteq> Some q)) \<and>
+    cee = ic_principal \<and>
+    mn = encode_string ''install_code'' \<and>
+    (case candid_parse_cid d of Some cid \<Rightarrow>
+    (case (candid_parse_text d [encode_string ''mode''], candid_parse_blob d [encode_string ''wasm_module''], candid_parse_blob d [encode_string ''arg'']) of
+      (Some mode, Some w, Some a) \<Rightarrow>
+    (case parse_wasm_mod w of Some m \<Rightarrow>
+    (case (list_map_get (canisters S) cid, list_map_get (controllers S) cid, list_map_get (time S) cid, list_map_get (balances S) cid, list_map_get (canister_status S) cid) of
+      (Some (Some can), Some ctrls, Some t, Some bal, Some can_status) \<Rightarrow>
+      let env = \<lparr>env_time = t, balance = bal, freezing_limit = ic_freezing_limit S cid, certificate = None, status = simple_status can_status\<rparr> in
+      (mode = encode_string ''upgrade'') \<and>
+      cer \<in> ctrls \<and>
+      (case canister_module_pre_upgrade (module can) (wasm_state can, cer, env) of Inr pre_ret \<Rightarrow>
+      (case canister_module_post_upgrade m (cid, cycles_return.return pre_ret, a, cer, env) of Inr post_ret \<Rightarrow>
+        cycles_return.cycles_used pre_ret + cycles_return.cycles_used post_ret \<le> bal
+      | _ \<Rightarrow> False) | _ \<Rightarrow> False)
+    | _ \<Rightarrow> False) | _ \<Rightarrow> False) | _ \<Rightarrow> False) | _ \<Rightarrow> False)
+  | _ \<Rightarrow> False))"
+
+definition ic_code_upgrade_post :: "nat \<Rightarrow> nat \<Rightarrow> ('p, 'uid, 'canid, 'b, 'w, 'sm, 'c, 's, 'cid, 'pk) ic \<Rightarrow> ('p, 'uid, 'canid, 'b, 'w, 'sm, 'c, 's, 'cid, 'pk) ic" where
+  "ic_code_upgrade_post n memory S = (case messages S ! n of Call_message orig cer cee mn d trans_cycles q \<Rightarrow>
+    let cid = the (candid_parse_cid d) in
+    (case candid_parse_cid d of Some cid \<Rightarrow>
+    (case (candid_parse_text d [encode_string ''mode''], candid_parse_blob d [encode_string ''wasm_module''], candid_parse_blob d [encode_string ''arg'']) of
+      (Some mode, Some w, Some a) \<Rightarrow>
+    (case parse_wasm_mod w of Some m \<Rightarrow>
+    (case (list_map_get (canisters S) cid, list_map_get (time S) cid, list_map_get (balances S) cid, list_map_get (canister_status S) cid) of
+      (Some (Some can), Some t, Some bal, Some can_status) \<Rightarrow>
+      let env = \<lparr>env_time = t, balance = bal, freezing_limit = ic_freezing_limit S cid, certificate = None, status = simple_status can_status\<rparr> in
+      (case canister_module_pre_upgrade (module can) (wasm_state can, cer, env) of Inr pre_ret \<Rightarrow>
+      (case canister_module_post_upgrade m (cid, cycles_return.return pre_ret, a, cer, env) of Inr post_ret \<Rightarrow>
+    S\<lparr>canisters := list_map_set (canisters S) cid (Some \<lparr>wasm_state = cycles_return.return post_ret, module = m, raw_module = w,
+        public_custom_sections = the (parse_public_custom_sections w), private_custom_sections = the (parse_private_custom_sections w)\<rparr>),
+      balances := list_map_set (balances S) cid (bal - (cycles_return.cycles_used pre_ret + cycles_return.cycles_used post_ret)),
+      messages := take n (messages S) @ drop (Suc n) (messages S) @ [Response_message orig (Reply (blob_of_candid Candid_empty)) trans_cycles]\<rparr>)))))))"
+
+definition ic_code_upgrade_burned_cycles :: "nat \<Rightarrow> nat \<Rightarrow> ('p, 'uid, 'canid, 'b, 'w, 'sm, 'c, 's, 'cid, 'pk) ic \<Rightarrow> nat" where
+  "ic_code_upgrade_burned_cycles n memory S = (case messages S ! n of Call_message orig cer cee mn d trans_cycles q \<Rightarrow>
+    let cid = the (candid_parse_cid d) in
+    (case candid_parse_cid d of Some cid \<Rightarrow>
+    (case (candid_parse_text d [encode_string ''mode''], candid_parse_blob d [encode_string ''wasm_module''], candid_parse_blob d [encode_string ''arg'']) of
+      (Some mode, Some w, Some a) \<Rightarrow>
+    (case parse_wasm_mod w of Some m \<Rightarrow>
+    (case (list_map_get (canisters S) cid, list_map_get (time S) cid, list_map_get (balances S) cid, list_map_get (canister_status S) cid) of
+      (Some (Some can), Some t, Some bal, Some can_status) \<Rightarrow>
+      let env = \<lparr>env_time = t, balance = bal, freezing_limit = ic_freezing_limit S cid, certificate = None, status = simple_status can_status\<rparr> in
+      (case canister_module_pre_upgrade (module can) (wasm_state can, cer, env) of Inr pre_ret \<Rightarrow>
+      (case canister_module_post_upgrade m (cid, cycles_return.return pre_ret, a, cer, env) of Inr post_ret \<Rightarrow>
+      cycles_return.cycles_used pre_ret + cycles_return.cycles_used post_ret)))))))"
+
+lemma ic_code_upgrade_cycles_inv:
+  assumes "ic_code_upgrade_pre n S"
+  shows "total_cycles S = total_cycles (ic_code_upgrade_post n memory S) + ic_code_upgrade_burned_cycles n memory S"
+proof -
+  obtain orig cer cee mn d trans_cycles q where msg: "messages S ! n = Call_message orig cer cee mn d trans_cycles q"
+    using assms
+    by (auto simp: ic_code_upgrade_pre_def split: message.splits)
+  define older where "older = take n (messages S)"
+  define younger where "younger = drop (Suc n) (messages S)"
+  have msgs: "messages S = older @ Call_message orig cer cee mn d trans_cycles q # younger" "(older @ w # younger) ! n = w"
+    "take n older = older" "take (n - length older) ws = []" "drop (Suc n) older = []"
+    "drop (Suc n - length older) (w # ws) = ws" for w ws
+    using id_take_nth_drop[of n "messages S"] assms
+    by (auto simp: ic_code_upgrade_pre_def msg younger_def older_def nth_append)
+  show ?thesis
+    using assms list_map_sum_in_ge[where ?f="balances S" and ?g=id and ?x="the (candid_parse_cid d)"]
+    by (auto simp: ic_code_upgrade_pre_def ic_code_upgrade_post_def ic_code_upgrade_burned_cycles_def total_cycles_def Let_def msgs list_map_sum_in[where ?f="balances S"] split: message.splits option.splits sum.splits)
+qed
+
 end
 
 export_code request_submission_pre request_submission_post
@@ -1088,6 +1164,7 @@ export_code request_submission_pre request_submission_post
   ic_update_settings_pre ic_update_settings_post
   ic_canister_status_pre ic_canister_status_post
   ic_code_installation_pre ic_code_installation_post
+  ic_code_upgrade_pre ic_code_upgrade_post
 in Haskell module_name IC file_prefix code
 
 end
